Domain.lean
@@ -125,4 +125,5 @@ import Domain.Neighborhood.Theorem614
 import Domain.Neighborhood.Lemma615
 import Domain.Neighborhood.Theorem616
 import Domain.Neighborhood.Exercise617
+import Domain.Neighborhood.Exercise617Gen
 import Domain.InfoSys
